bakcup for new value def

CoqCode/Language.v
@@ -1,11 +1,16 @@
 Require Import Metalib.Metatheory.
 Require Import Coq.Program.Equality.
+Require Import Coq.Lists.List.
+
+Import ListNotations.
+
+Set Printing Parentheses.
 
 Inductive typ : Set :=
 | typ_int
 | typ_top
-| typ_arrow (A:typ) (B:typ)
-| typ_and (A:typ) (B:typ).
+| typ_arrow (A : typ) (B : typ)
+| typ_and (A : typ) (B : typ).
 
 Hint Constructors typ : core.
 
@@ -19,7 +24,7 @@ Inductive trm : Set :=
 | trm_merge : trm -> trm -> trm
 | trm_anno : trm -> typ -> trm.
 
-(* term is locally closed *)
+Coercion trm_fvar : atom >-> trm.
 
 Definition ctx : Set := list (var * typ).
 
@@ -53,14 +58,19 @@ Inductive term : trm -> Prop :=
 Hint Constructors trm : core.
 Hint Constructors term : core.
 
-Inductive value : trm -> Prop :=
-| value_top : value trm_top
-| value_nat : forall (n : nat), value (trm_nat n)
-| value_abs : forall (e : trm),
-    term (trm_abs e) -> value (trm_abs e)
-| value_merge : forall (e1 e2 : trm),
-    value e1 -> value e2 -> value (trm_merge e1 e2).
+Inductive pvalue : trm -> Prop :=
+| pvalue_top : pvalue trm_top
+| pvalue_nat : forall (n : nat), pvalue (trm_nat n)
+| pvalue_abs : forall (e : trm), term (trm_abs e) -> pvalue (trm_abs e)
+| pvalue_merge : forall (p1 p2 : trm), pvalue p1 -> pvalue p2 -> pvalue (trm_merge p1 p2).
 
+Inductive value : trm -> Prop :=
+| value_anno : forall (A : typ) (e : trm),
+    pvalue e -> value (trm_anno e A)
+| value_abs : forall (e : trm),
+    term (trm_abs e) -> value (trm_abs e).
+
+Hint Constructors pvalue : core.
 Hint Constructors value : core.
 
 Inductive toplike : typ -> Prop :=
@@ -70,7 +80,6 @@ Inductive toplike : typ -> Prop :=
 
 Hint Constructors toplike : core.
 
-(* ordinary types are those types aren't intersection *)
 Inductive ordinary : typ -> Prop :=
 | ord_top : ordinary typ_top
 | ord_int : ordinary typ_int
@@ -106,43 +115,60 @@ Fixpoint typ_stack (S : arg) (A : typ) : typ :=
 
 (* Compute (typ_stack (cons type_int (cons type_int nil)) type_top). *)
 
+Fixpoint next_inputs (A : typ) : list typ :=
+  match A with
+  | typ_top => [typ_top]
+  | typ_int => [typ_int]
+  | typ_arrow B C => [B]
+  | typ_and B C => (next_inputs B) ++ (next_inputs C)
+  end.
+
 (* S |- A <: B *)
 Inductive appsub : arg -> typ -> typ -> Prop :=
 | as_refl : forall (A : typ),
     appsub nil A A
-| as_top : forall (A : typ),
-    appsub nil A typ_top
+(* | as_top : forall (A : typ), *)
+(*     appsub nil A typ_top *)
 | as_fun : forall (C A B D : typ) (S : arg),
     sub C A ->
     appsub S B D ->
     appsub (cons C S) (typ_arrow A B) (typ_arrow C D)
-| as_and_l : forall (A B D: typ) (S : arg),
+| as_and_l : forall (A B C D: typ) (S : arg),
     appsub S A D ->
-    not (sub B (typ_stack S typ_top)) ->
-    appsub S (typ_and A B) D
-| as_and_r : forall (A B D: typ) (S : arg),
+    not (In C (next_inputs B)) ->
+    appsub (cons C S) (typ_and A B) D
+| as_and_r : forall (A B C D: typ) (S : arg),
     appsub S B D ->
-    not (sub A (typ_stack S typ_top)) ->
-    appsub S (typ_and A B) D.
+    not (In C (next_inputs A)) ->
+    appsub (cons C S) (typ_and A B) D.
 
 Hint Constructors appsub : core.
 
 Inductive typedred : trm -> typ -> trm -> Prop :=
 | tred_int : forall (n : nat),
-    typedred (trm_nat n) typ_int (trm_nat n)
-| tred_top : forall (A : typ) (e : trm),
-    term e -> toplike A -> ordinary A -> typedred e A trm_top
-| tred_arrow_anno : forall (A B C D : typ) (e : trm), (* A -> B <: C -> D *)
-    term (trm_abs e) -> not (toplike D) -> sub C A -> sub B D ->
+    typedred (trm_anno (trm_nat n) typ_int) typ_int (trm_anno (trm_nat n) typ_int)
+| tred_top : forall (A : typ) (v : trm),
+    value v ->
+    toplike A -> ordinary A ->
+    typedred v A (trm_anno trm_top typ_top)
+| tred_arrow_anno : forall (A B C D : typ) (e : trm),
+    not (toplike D) -> sub C A -> sub B D ->
     typedred (trm_anno (trm_abs e) (typ_arrow A B))
              (typ_arrow C D)
              (trm_anno (trm_abs e) (typ_arrow A D))
-| tred_merge_l : forall (e1 e1' e2 : trm) (A : typ),
-    term e2 -> typedred e1 A e1' -> ordinary A -> typedred (trm_merge e1 e2) A e1'
-| tred_merge_r : forall (e1 e2 e2' : trm) (A : typ),
-    term e1 -> typedred e2 A e2' -> ordinary A -> typedred (trm_merge e1 e2) A e2'
-| tred_and : forall (e1 e2 e3 : trm) (A B: typ),
-    typedred e1 A e2 -> typedred e1 B e3 -> typedred e1 (typ_and A B) (trm_merge e2 e3).
+| tred_merge_l : forall (p1 p2 p: trm) (A B C D : typ),
+    pvalue p1 -> pvalue p2 -> pvalue p ->
+    typedred (trm_anno p1 A) C (trm_anno p D) -> ordinary C ->
+    typedred (trm_anno (trm_merge p1 p2) (typ_and A B)) C (trm_anno p D)
+| tred_merge_r : forall (p1 p2 p : trm) (A B C D : typ),
+    pvalue p1 -> pvalue p2 -> pvalue p ->
+    typedred (trm_anno p2 B) C (trm_anno p D) -> ordinary C ->
+    typedred (trm_anno (trm_merge p1 p2) (typ_and A B)) C (trm_anno p D)
+| tred_and : forall (p1 p2 p : trm) (A B C D E : typ),
+    pvalue p1 -> pvalue p2 -> pvalue p ->
+    typedred (trm_anno p C) A (trm_anno p1 D) ->
+    typedred (trm_anno p C) B (trm_anno p2 E) ->
+    typedred (trm_anno p C) (typ_and A B) (trm_anno (trm_merge p1 p2) (typ_and D E)).
 
 Hint Constructors typedred : core.
 
@@ -164,6 +190,11 @@ Hint Constructors disjoint : core.
 
 Definition disjoint_spec A B :=
   forall (C : typ), sub A C -> sub B C -> toplike C.
+
+Inductive hastype : trm -> Prop :=
+| ht_int : forall (n : nat), hastype (trm_nat n)
+| ht_top : hastype trm_top
+| ht_merge : forall (e1 e2 : trm), hastype (trm_merge e1 e2).
 
 Inductive typing : ctx -> arg -> mode -> trm -> typ -> Prop :=
 | typing_int : forall (T: ctx) (n : nat),
@@ -197,30 +228,61 @@ Inductive typing : ctx -> arg -> mode -> trm -> typ -> Prop :=
     disjoint_spec A B ->
     typing T nil infer_mode e1 A ->
     typing T nil infer_mode e2 B ->
-    typing T nil infer_mode (trm_merge e1 e2) (typ_and A B).
+    typing T nil infer_mode (trm_merge e1 e2) (typ_and A B)
+| typing_merge_chk : forall (A B : typ) (e1 e2 : trm),
+    disjoint_spec A B ->
+    not (hastype (trm_merge e1 e2)) ->
+    typing nil nil check_mode e1 A ->
+    typing nil nil check_mode e2 B ->
+    typing nil nil check_mode (trm_merge e1 e2) (typ_and A B).
+
 
 Hint Constructors typing : core.
 
 Parameter Y : atom.
-Compute (open (trm_abs (trm_bvar 0)) (trm_fvar Y)).
+
+Inductive papp : trm -> trm -> trm -> Prop :=
+| papp_top : forall (v : trm),
+    papp trm_top v trm_top
+| papp_abs : forall (e v : trm),
+    papp (trm_abs e) v (open e v)
+| papp_abs_anno : forall (A B : typ) (e v v' : trm),
+    typedred v A v' ->
+    papp (trm_anno (trm_abs e) (typ_arrow A B)) v
+         (trm_anno (open e v') B)
+| papp_merge : forall (A B C D : typ) (p1 p2 p e v : trm),
+    appsub (cons C nil) (typ_and A B) D ->
+    typedred (trm_anno (trm_merge p1 p2) (typ_and A B)) D v ->
+    papp v (trm_anno p C) e ->
+    papp (trm_anno (trm_merge p1 p2) (typ_and A B))
+         (trm_anno p C) e.
 
 Inductive step : trm -> trm -> Prop :=
-| step_top : forall (e : trm),
-    value e -> step (trm_app trm_top e) trm_top
-| step_beta : forall (e1 e2 e2' : trm) (A B : typ),
-    term (trm_abs e1) -> value e2 -> typered e2 A e2' ->
-    step (trm_app (trm_abs e1) e2) (open e1 e2')
-| step_anno_typed : forall (e e' : trm) (A : typ),
-    value e -> typedred e A e' -> step (trm_anno e A) e'
-| step_app_l : forall (e1 e2 e1' : trm),
-    term e2 -> step e1 e1' -> step (trm_app e1 e2) (trm_app e1' e2)
-| step_app_r : forall (e1 e2 e2' : trm),
-    value e1 -> step e2 e2' -> step (trm_app e1 e2) (trm_app e1 e2')
-| step_merge_l : forall (e1 e2 e1' : trm),
-    term e2 -> step e1 e1' -> step (trm_merge e1 e2) (trm_merge e1' e2)
-| step_merge_r : forall (e1 e2 e2' : trm),
-    value e2 -> step e2 e2' -> step (trm_merge e1 e2) (trm_merge e1 e2')
+| step_int_anno : forall (n : nat),
+    step (trm_nat n) (trm_anno (trm_nat n) typ_int)
+| step_papp : forall (v1 v2 e : trm),
+    value v1 -> value v2 -> papp v1 v2 e ->
+    step (trm_app v1 v2) e
+| step_anno_value : forall (v v' : trm) (A : typ),
+    value v -> typedred v A v' ->
+    step (trm_anno v A) v'
 | step_anno : forall (e e' : trm) (A : typ),
-    step e e' -> step (trm_anno e A) (trm_anno e' A).
+    not (value (trm_anno e A)) ->
+    step e e' -> step (trm_anno e A) (trm_anno e' A)
+| step_app_l : forall (e1 e2 e1' : trm),
+    step e1 e1' -> step (trm_app e1 e2) (trm_app e1' e2)
+| step_app_r : forall (v e2 e2' : trm),
+    value v -> step e2 e2' -> step (trm_app v e2) (trm_app v e2')
+| step_merge_anno : forall (e1 e2 : trm) (A B : typ),
+    step (trm_merge (trm_anno e1 A) (trm_anno e2 B))
+         (trm_anno (trm_merge e1 e2) (typ_and A B))
+| step_merge_l : forall (e1 e2 e : trm) (A B C : typ),
+    step (trm_anno e1 A) (trm_anno e C) ->
+    step (trm_anno (trm_merge e1 e2) (typ_and A B))
+         (trm_anno (trm_merge e e2) (typ_and C B))
+| step_merge_r : forall (p1 e2 e: trm) (A B C : typ),
+    pvalue p1 -> step (trm_anno e2 B) (trm_anno e C) ->
+    step (trm_anno (trm_merge p1 e2) (typ_and A B))
+         (trm_anno (trm_merge p1 e) (typ_and A C)).
 
 Hint Constructors step : core.
