CoqCode/Deterministic.v
@@ -1,0 +1,169 @@
+Require Import Coq.Program.Equality.
+Require Import Language Notations Auxiliaries Subtyping.
+Require Import Strings.String.
+
+Set Printing Parentheses.
+
+Lemma tred_ord_toplike : forall (e e' : trm) (A : typ),
+    ordinary A -> toplike A -> typedred e A e' -> e' = (trm_anno trm_top typ_top).
+Proof.
+  intros e e' A H_ord H_top H_tred.
+  dependent induction H_tred; subst; eauto.
+  - inversion H_top.
+  - inversion H_top. contradiction.
+  - inversion H_ord.
+Qed.
+
+Lemma tred_toplike :
+  forall (A : typ),
+    toplike A -> forall e1 e2 e1' e2' : trm, typedred e1 A e1' -> typedred e2 A e2' -> e1' = e2'.
+Proof.
+  intros A Htop.
+  dependent induction Htop; intros e1 e2 e1' e2' H_tred1 H_tred2.
+  - eapply tred_ord_toplike in H_tred1. eapply tred_ord_toplike in H_tred2.
+    rewrite H_tred1. rewrite H_tred2. reflexivity.
+    constructor. constructor. constructor. constructor.
+  - inversion H_tred1; subst; eauto 3.
+    + inversion H1.
+    + inversion H3.
+    + inversion H3.
+    + inversion H_tred2; subst; eauto 3.
+      * inversion H4.
+      * inversion H8.
+      * inversion H8.
+      * assert (Heq1: (trm_anno p1 D) = (trm_anno p0 D0)).
+        eapply IHHtop1; eauto 3.
+        assert (Heq2: (trm_anno p2 E) = (trm_anno p3 E0)).
+        eapply IHHtop2; eauto 3.
+        eapply anno_equal_split in Heq1.
+        destruct Heq1 as [Heq11 Heq12].
+        eapply anno_equal_split in Heq2.
+        destruct Heq2 as [Heq21 Heq22].
+        rewrite Heq11. rewrite Heq12. rewrite Heq21. rewrite Heq22. reflexivity.
+  - assert (HAB: toplike (typ_arrow A B)).
+    constructor. assumption.
+    eapply tred_ord_toplike in H_tred2; eauto.
+    eapply tred_ord_toplike in H_tred1; eauto.
+    rewrite H_tred1. rewrite H_tred2. reflexivity.
+Qed.
+
+Lemma toplike_sub_top :
+  forall (A : typ),
+    toplike A <-> sub typ_top A.
+Proof.
+  intro A. split.
+  - intro H. induction H.
+    + constructor.
+    + constructor. assumption. assumption.
+    + constructor. assumption.
+  - intro H. induction A; eauto.
+    + inversion H; subst; eauto.
+    + inversion H; subst. constructor.
+      apply IHA2. assumption.
+    + constructor; inversion H; subst.
+      apply IHA1. assumption.
+      apply IHA2. assumption.
+Qed.
+
+Lemma tred_sub :
+  forall (A B : typ) (v1 v2 : trm),
+    value v1 -> typedred v1 A v2 ->
+    typing nil nil infer_mode v1 B ->
+    sub B A.
+Proof.
+  intros A B v1 v2 Hval Hred Htyp.
+  generalize dependent B.
+  induction Hred; eauto.
+  - intros B Htyp.
+    inversion Htyp; subst.
+    inversion H3; subst. constructor.
+  - intros B Htyp.
+    eapply toplike_sub_top in H0.
+    eapply sub_transitivity.
+    constructor. assumption.
+  - intros B0 Htyp.
+    inversion Hval; subst; clear Hval.
+    inversion Htyp; subst; clear Htyp.
+    inversion H7; subst.
+    apply sub_arrow. assumption. assumption.
+  - intros B0 Htyp.
+    inversion Htyp; subst; clear Htyp.
+    inversion H7; subst; clear H7.
+    apply sub_and_l.
+    eapply IHHred. constructor. assumption.
+    inversion H8; subst.
+    Focus 2.
+    + apply typing_anno. constructor. assumption.
+Admitted.
+  (* pose proof (tred_to_sub e1 e1' A0 A) as Hsub1. *)
+  (* apply Hsub1. assumption. assumption. assumption. *)
+  (* pose proof (tred_to_sub e2 e2' A0 B) as Hsub2. *)
+  (* apply Hsub2. assumption. assumption. assumption. *)
+  (* apply tred_toplike with (A:=A0) (e1:=e1) (e2:=e2). *)
+(*   (* assumption. assumption. assumption. *) *)
+(* Qed. *)
+
+Lemma tred_determinism :
+  forall (v v1 v2 : trm) (A : typ),
+    value v -> (exists B, typing nil nil infer_mode v B) ->
+    typedred v A v1 -> typedred v A v2 -> v1 = v2.
+Proof.
+  intros v v1 v2 A Hval Htyp Hred1.
+  generalize dependent v2.
+  induction Hred1.
+  - intros v2 Hred2. inversion Hred2; subst.
+    + reflexivity.
+    + inversion H0.
+  - intros v2 Hred2.
+    inversion Hred2; subst; clear Hred2.
+    + inversion H0.
+    + reflexivity.
+    + inversion H0. contradiction.
+    + symmetry. eapply tred_ord_toplike; eauto.
+    + symmetry. eapply tred_ord_toplike; eauto.
+    + inversion H1.
+  - intros v2 Hred2.
+    inversion Hred2; subst; clear Hred2.
+    + inversion H3. contradiction.
+    + reflexivity.
+  - intros v2 Hred2.
+    inversion Hred2; subst; eauto.
+    + eapply tred_ord_toplike; eauto 3.
+    + eapply IHHred1.
+      * constructor. assumption.
+      * destruct Htyp. inversion H3; subst.
+        inversion H14; subst.
+        inversion H4; subst.
+        inversion H5; subst.
+        unfold disjoint_spec in H15.
+    (* + assert (Hval1 : value (trm_anno p1 A)). constructor. assumption. *)
+    (*   eapply IHHred1 in Hval1. apply Hval1. *)
+Admitted.
+
+Lemma papp_determinism :
+  forall (v1 v2 e1 e2 : trm),
+    papp v1 v2 e1 -> papp v1 v2 e2 -> e1 = e2.
+Proof.
+  intros v1 v2 e1 e2 Hp1.
+  generalize dependent e2.
+  induction Hp1.
+  - intros e2 Hp2. inversion Hp2. reflexivity.
+  - intros e2 Hp2. inversion Hp2. reflexivity.
+  - intros e2 Hp2. inversion Hp2; subst.
+    Admitted.
+
+Lemma step_determinism :
+  forall (e e1 e2 : trm) (A : typ),
+    typing nil nil check_mode e A ->
+    step e e1 -> step e e2 -> e1 = e2.
+Proof.
+  intros e e1 e2 A Htyp Hred1.
+  generalize dependent e2.
+  generalize dependent A.
+  induction Hred1.
+  - intros A Htyp e2 Hred2.
+    inversion Hred2; subst.
+    reflexivity.
+  - intros A0 Htyp e2 Hred2.
+    inversion Hred2; subst.
+Admitted.
