CoqCode/Notations.v
@@ -1,5 +1,7 @@
 Require Import Language.
 
+Notation "e ∷ A" := (trm_anno e A) (at level 20).
+
 Notation "A → B" := (typ_arrow A B) (at level 20).
 Notation "A & B" := (typ_and A B) (at level 20).
 (* Notation "⌉ A ⌈" := (toplike A) (at level 30). *)
@@ -10,7 +12,7 @@ Notation "A & B" := (typ_and A B) (at level 20).
 Notation "A <: B" := (sub A B) (at level 40).
 Notation "S ⤞ A" := (typ_stack S A) (at level 40).
 Notation "S ⊢ A <: B" := (appsub S A B) (at level 40).
-Notation "e ~-> A e'" := (typedred e A e') (at level 68).
+Notation "e ~->> A e'" := (typedred e A e') (at level 68).
 
 Notation "T S ⊢ e ⇒ A" := (typing T S infer_mode e A) (at level 50).
 Notation "T S ⊢ e ⇐ A" := (typing T S check_mode e A) (at level 50).
