CoqCode/Soundness.v
@@ -1,0 +1,87 @@
+Require Import Metalib.Metatheory.
+Require Import Coq.Program.Equality.
+Require Import Language Subtyping Notations.
+
+Inductive runsub : typ -> typ -> Prop :=
+| rsub_refl : forall (A : typ),
+    runsub A A
+| rsub_arrow : forall (A1 A2 B1 B2 : typ),
+    sub B1 A1 -> runsub A2 B2 ->
+    runsub (typ_arrow A1 A2) (typ_arrow B1 B2)
+| rsub_and : forall (A1 A2 B1 B2 : typ),
+    runsub A1 B1 -> runsub A2 B2 ->
+    runsub (typ_and A1 A2) (typ_and B1 B2)
+| rsub_top : forall (A : typ),
+    toplike A -> runsub typ_top A.
+
+Lemma typing_sub_check :
+  forall (e : trm) (A B : typ),
+    typing nil nil check_mode e A ->
+    sub A B ->
+    typing nil nil check_mode e B.
+Proof.
+  intros e A B Htyp Hsub.
+  dependent induction Hsub; eauto.
+  - inversion Htyp; subst.
+    inversion Htyp; subst.
+Admitted.
+
+Theorem tred_preservation :
+  forall (v v' : trm) (A: typ),
+    value v -> typing nil nil check_mode v A ->
+    typedred v A v' ->
+    exists (B : typ), typing nil nil infer_mode v' B /\ runsub B A.
+Proof.
+  intros v v' A B.
+  intros Htyp Hred.
+  dependent induction Hred.
+  - exists typ_int. split.
+    + apply typing_anno.
+      apply as_refl.
+      apply typing_sub with (B:=typ_int).
+      apply typing_int. constructor. apply sub_reflexivity.
+    + apply rsub_refl.
+  - exists typ_top. split.
+    + apply typing_anno.
+      apply as_refl.
+      apply typing_sub with (B:=typ_top).
+      apply typing_top. apply sub_reflexivity.
+    + apply rsub_top. assumption.
+  - exists (typ_arrow A D). split.
+    Focus 2.
+    + apply rsub_arrow. assumption. apply rsub_refl.
+    + apply typing_anno.
+      apply as_refl.
+      inversion Htyp; subst; clear Htyp.
+      inversion H2; subst; clear H2.
+      inversion H8; subst; clear H8.
+      inversion H3; subst.
+      Focus 2.
+      eapply typing_abs1.
+      intros.
+      (* inversion Htyp; subst. inversion H3; subst. *)
+      (* inversion H10; subst. *)
+      (* specialize (H11 x). *)
+Admitted.
+
+Theorem preservation :
+  forall (e e' : trm) (A : typ),
+    typing nil nil infer_mode e A ->
+    step e e' ->
+    typing nil nil check_mode e' A.
+Proof.
+  intros e e' A Htyp Hred.
+  induction Htyp.
+  - inversion Hred; subst.
+    apply typing_sub with (B:=typ_int).
+    apply typing_anno. constructor.
+    apply typing_sub with (B:=typ_int).
+    apply typing_int. assumption. apply sub_reflexivity. apply sub_reflexivity.
+  - inversion Hred.
+  - inversion Hred.
+  - inversion Hred.
+  - inversion Hred.
+  - inversion Hred; subst.
+    + induction A; eauto.
+      * inversion H; subst; clear H.
+Admitted.
