CoqCode/TypedRedudction.v
@@ -2,115 +2,63 @@ Require Import Metalib.Metatheory.
 Require Import Coq.Program.Equality.
 Require Import Language Subtyping Auxiliaries Notations.
 
-Lemma tred_ord_toplike_normal : forall (e e' : trm) (A : typ),
-    ordinary A -> toplike A -> typedred e A e' -> e' = trm_top.
-Proof.
-  intros e e' A H_ord H_top H_tred.
-  dependent induction H_tred; subst; eauto.
-  - inversion H_top.
-  - destruct H0. inversion H_top; subst.
-    assumption.
-  - inversion H_ord.
-Qed.
 
-Lemma tred_toplike :
-  forall (A : typ),
-    toplike A -> forall e1 e2 e1' e2' : trm, typedred e1 A e1' -> typedred e2 A e2' -> e1' = e2'.
-Proof.
-  intros A Htop.
-  dependent induction Htop; intros e1 e2 e1' e2' H_tred1 H_tred2.
-  - apply tred_ord_toplike_normal with (A:=typ_top) in H_tred1; auto; subst.
-    apply tred_ord_toplike_normal with (A:=typ_top) in H_tred2; auto; subst.
-  - inversion H_tred1; subst; eauto.
-    + inversion H1.
-    + inversion H1.
-    + inversion H1.
-    + inversion H_tred2; subst; eauto; try (inversion H0); try (inversion H1).
-      assert (Heq1: e3 = e5).
-      pose proof (IHHtop1 e1 e2 e3 e5) as IHHtop1'.
-      apply IHHtop1'. assumption. assumption.
-      assert (Heq2: e4 = e6).
-      pose proof (IHHtop2 e1 e2 e4 e6) as IHHtop2'.
-      apply IHHtop2'. assumption. assumption.
-      rewrite Heq1. rewrite Heq2. reflexivity.
-  - assert (HAB: toplike (typ_arrow A B)).
-    constructor. assumption.
-    apply tred_ord_toplike_normal with (A:=(typ_arrow A B)) in H_tred2.
-    apply tred_ord_toplike_normal with (A:=(typ_arrow A B)) in H_tred1.
-    rewrite H_tred1. rewrite H_tred2. reflexivity.
-    constructor. assumption. constructor. assumption.
-Qed.
 
-Lemma toplike_sub_top : forall (A : typ),
-    toplike A <-> sub typ_top A.
-Proof.
-  intro A. split.
-  - intro H. induction H.
-    + constructor.
-    + constructor. assumption. assumption.
-    + constructor. assumption.
-  - intro H. induction A; eauto.
-    + inversion H; subst; eauto.
-    + inversion H; subst. constructor.
-      apply IHA2. assumption.
-    + constructor; inversion H; subst.
-      apply IHA1. assumption.
-      apply IHA2. assumption.
-Qed.
+(* Lemma tred_to_sub: forall (e e' : trm) (A B : typ), *)
+(*     value e -> typedred e A e' -> typing nil nil infer_mode e B -> sub B A. *)
+(* Proof. *)
+(*   intros e e' A B Hval Hred Htyp. *)
+(*   generalize dependent B. *)
+(*   induction Hred; eauto. *)
+(*   - intros B Htyp. *)
+(*     inversion Htyp; subst. inversion H3; subst. *)
+(*     + constructor. *)
+(*     + inversion Htyp; subst. *)
+(*   - intros B Htyp. *)
+(*     apply toplike_sub_top in H0. *)
+(*     pose proof (sub_transitivity typ_top B A) as sub_trans'. *)
+(*     assert (H_sub1: sub B typ_top). *)
+(*     constructor. apply sub_trans' in H_sub1. assumption. assumption. *)
+(*   - inversion Hval. *)
+(*   - intros B Htyp. *)
+(*     inversion Hval; inversion Htyp; subst. *)
+(*     apply sub_and_l. *)
+(*     apply IHHred. assumption. assumption. *)
+(*   - intros B Htyp. *)
+(*     inversion Hval; inversion Htyp; subst. *)
+(*     apply sub_and_r. *)
+(*     apply IHHred. assumption. assumption. *)
+(* Qed. *)
 
-Lemma tred_to_sub: forall (e e' : trm) (A B : typ),
-    value e -> typedred e A e' -> typing nil nil infer_mode e B -> sub B A.
-Proof.
-  intros e e' A B Hval Hred Htyp.
-  generalize dependent B.
-  induction Hred; eauto.
-  - intros B Htyp.
-    inversion Htyp; subst. constructor.
-  - intros B Htyp.
-    apply toplike_sub_top in H0.
-    pose proof (sub_transitivity typ_top B A) as sub_trans'.
-    assert (H_sub1: sub B typ_top).
-    constructor. apply sub_trans' in H_sub1. assumption. assumption.
-  - inversion Hval.
-  - intros B Htyp.
-    inversion Hval; inversion Htyp; subst.
-    apply sub_and_l.
-    apply IHHred. assumption. assumption.
-  - intros B Htyp.
-    inversion Hval; inversion Htyp; subst.
-    apply sub_and_r.
-    apply IHHred. assumption. assumption.
-Qed.
-
-Lemma tred_transitivity : forall (e1 e2 e3: trm) (A B : typ),
-    value e1 -> typedred e1 A e2 -> typedred e2 B e3 -> typedred e1 B e3.
-Proof.
-  intros e1 e2 e3 A B Hval Hred1 Hred2.
-  generalize dependent e3.
-  generalize dependent B.
-  dependent induction Hred1; eauto.
-  - intros B e3 Hred2. dependent induction Hred2; eauto.
-  - intros B0 e3 Hred2. dependent induction Hred2; eauto.
-    + constructor. assumption. assumption. assumption.
-      pose proof (sub_transitivity D B D0) as Hsub.
-      apply Hsub in H2. assumption. assumption.
-  - intros B e3 Hred2.
-    inversion Hval; subst; clear Hval.
-    induction Hred2; eauto.
-  - intros B e3 Hred2. inversion Hval; subst; clear Hval.
-    induction Hred2; eauto.
-  - intros B0 e0 Hred2.
-    generalize dependent e0.
-    induction B0; intros e0 Hred2; eauto.
-    + inversion Hred2; subst; clear Hred2; eauto.
-      * inversion H0.
-    + inversion Hred2; subst; clear Hred2; eauto.
-      * apply tred_top. apply value_to_term in Hval. assumption. assumption. assumption.
-    + inversion Hred2; subst; clear Hred2; eauto.
-      * apply tred_top. apply value_to_term in Hval. assumption. assumption. assumption.
-    + inversion Hred2; subst; clear Hred2; eauto.
-      * constructor. apply value_to_term in Hval. assumption. assumption. assumption.
-Qed.
+(* Lemma tred_transitivity : forall (e1 e2 e3: trm) (A B : typ), *)
+(*     value e1 -> typedred e1 A e2 -> typedred e2 B e3 -> typedred e1 B e3. *)
+(* Proof. *)
+(*   intros e1 e2 e3 A B Hval Hred1 Hred2. *)
+(*   generalize dependent e3. *)
+(*   generalize dependent B. *)
+(*   dependent induction Hred1; eauto. *)
+(*   - intros B e3 Hred2. dependent induction Hred2; eauto. *)
+(*   - intros B0 e3 Hred2. dependent induction Hred2; eauto. *)
+(*     + constructor. assumption. assumption. assumption. *)
+(*       pose proof (sub_transitivity D B D0) as Hsub. *)
+(*       apply Hsub in H2. assumption. assumption. *)
+(*   - intros B e3 Hred2. *)
+(*     inversion Hval; subst; clear Hval. *)
+(*     induction Hred2; eauto. *)
+(*   - intros B e3 Hred2. inversion Hval; subst; clear Hval. *)
+(*     induction Hred2; eauto. *)
+(*   - intros B0 e0 Hred2. *)
+(*     generalize dependent e0. *)
+(*     induction B0; intros e0 Hred2; eauto. *)
+(*     + inversion Hred2; subst; clear Hred2; eauto. *)
+(*       * inversion H0. *)
+(*     + inversion Hred2; subst; clear Hred2; eauto. *)
+(*       * apply tred_top. apply value_to_term in Hval. assumption. assumption. assumption. *)
+(*     + inversion Hred2; subst; clear Hred2; eauto. *)
+(*       * apply tred_top. apply value_to_term in Hval. assumption. assumption. assumption. *)
+(*     + inversion Hred2; subst; clear Hred2; eauto. *)
+(*       * constructor. apply value_to_term in Hval. assumption. assumption. assumption. *)
+(* Qed. *)
 
 Lemma disjoint_value_consistent : forall (A B : typ) (e1 e2 : trm),
     disjoint_spec A B -> value e1 -> value e2 -> typing nil nil infer_mode e1 A -> typing nil nil infer_mode e2 B ->
